BR93: cleanup, limiting smt, clarity.

examples/br93.ec
@@ -13,7 +13,10 @@ op k : { int | 0 < k } as gt0_k. (* size of plaintexts *)
 clone import BitWord as Plaintext with
   op n <- k
 proof gt0_n by exact/gt0_k
-rename "word" as "ptxt".
+rename
+  "word" as "ptxt"
+  "dunifin" as "dptxt".
+import DWord.
 
 (** A type for nonces **)
 op l : { int | 0 < l } as gt0_l. (* size of nonces *)
@@ -21,7 +24,10 @@ op l : { int | 0 < l } as gt0_l. (* size of nonces *)
 clone import BitWord as Randomness with
   op n <- l
 proof gt0_n by exact/gt0_l
-rename "word" as "rand".
+rename
+  "word" as "rand"
+  "dunifin" as "drand".
+import DWord.
 
 (** A type for ciphertexts **)
 op n = k + l.                    (* size of ciphertexts *)
@@ -31,10 +37,6 @@ clone import BitWord as Ciphertext with
   op n <- n
 proof gt0_n by exact/Self.gt0_n
 rename "word" as "ctxt".
-
-(** We rename a few things to make them usable...                      **)
-op dptxt = Plaintext.DWord.dunifin.
-op drand = Randomness.DWord.dunifin.
 
 (** ... and define the concatenation of nonce and plaintext into
     a ciphertext.                                                      **)
@@ -52,8 +54,8 @@ clone import OW as OW_rand with
   type R           <- rand,
   op   challenge _ <- drand
 proof challenge_ll, challenge_uni.
-realize challenge_ll by move=> _ _; exact/Randomness.DWord.dunifin_ll.
-realize challenge_uni by move=> _ _; exact/Randomness.DWord.dunifin_uni.
+realize challenge_ll by move=> _ _; exact/drand_ll.
+realize challenge_uni by move=> _ _; exact/drand_uni.
 (** f is a secure OWTP if, for any inverter I,
       Adv^{OW}^f(I) = Pr[OW(I).main() @ &m: res]
     is small. **)
@@ -80,7 +82,7 @@ module type Scheme(RO : Oracle) = {
   proc enc(pk:pkey, m:ptxt): ctxt
 }.
 
-module type Adv(ARO: ARO)  = {
+module type Adv (ARO: ARO)  = {
   proc a1(p:pkey): (ptxt * ptxt)
   proc a2(c:ctxt): bool
 }.
@@ -102,8 +104,7 @@ module CPA(S:Scheme, A:Adv) = {
     return b' = b;
   }
 }.
-
-(** A Scheme E is IND-CPA secure if, for any A,
+(** A PKE Scheme E is IND-CPA secure if, for any A,
       Adv^{CPA}_{S}(A) = `|Pr[CPA(S,A).main() @ &m: res] - 1/2|
     is small. **)
 
@@ -145,20 +146,20 @@ module BR_OW(A:Adv): Inverter = {
   }
 }.
 
-(** such that Adv^{CPA}_{S}(A) <= Adv^{OW}^{f}(I(A)).
-    We now prove this bound. **)
 lemma ARO_init_ll: islossless Log(RO).init.
 proof. by apply/(Log_init_ll RO)/RO_init_ll. qed.
 
 lemma ARO_o_ll : islossless Log(RO).o.
-proof. by apply/(Log_o_ll RO)/RO_o_ll/Plaintext.DWord.dunifin_ll. qed.
+proof. by apply/(Log_o_ll RO)/RO_o_ll/dptxt_ll. qed.
 
+(** such that Adv^{CPA}_{S}(A) <= Adv^{OW}^{f}(I(A)).
+    We now prove this bound. **)
 section.
   (* Forall CPA adversary A whose memory footprint is disjoint from
      that of RO, Log and OW *)
   declare module A : Adv {RO,Log,OW}.
 
-  (* and whose two procedures as lossless provided the random oracle is *)
+  (* and whose two procedures are lossless provided the random oracle is *)
   axiom a1_ll (O <: ARO{A}): islossless O.o => islossless A(O).a1.
   axiom a2_ll (O <: ARO{A}): islossless O.o => islossless A(O).a2.
 
@@ -188,36 +189,56 @@ section.
     <= Pr[CPA(BR1,A).main() @ &m: res]
        + Pr[CPA(BR1,A).main() @ &m: mem Log.qs BR1.r].
   proof.
-    byequiv=> //=.
-    proc.
-    (* Until the adversary queries the ROM with r, knowing that
-       the two ROMs agree on all points except r is sufficient
-       to prove the equivalence of the adversary's views        *)
-    call (_: mem Log.qs BR1.r ,
-             eq_except RO.m{1} RO.m{2} (pred1 BR1.r{2})).
-      (* Adversary is lossless *)
-      exact/a2_ll.
-      (* Oracles are equivalent up to the failure event *)
-      proc. inline RO.o.
-      wp. rnd.
-      wp. skip. smt (@NewFMap).
-      (* Left oracle is lossless *)
-      move=> &2 _; exact/ARO_o_ll.
-      (* Right oracle is lossless and preserves bad once set *)
-      move=> &1. proc. inline *. wp. rnd. wp. skip. smt. (* or use conseq [-frame]... *)
-    (* We return to the main game *)
-    inline CPA(BR,A).SO.enc CPA(BR1,A).SO.enc.
-    inline RO.o.
-    wp. rnd.
-    wp. rnd.
-    wp. rnd.
-    (* The first adversary call is simpler *)
-    call (_:    ={Log.qs, RO.m}
-             /\ (forall x, mem Log.qs{1} x <=> mem (dom RO.m){1} x)).
-      proc. inline RO.o.
-      wp. rnd.
-      wp. skip=> /> &2 log_is_dom y _; smt(@NewFMap).
-    inline *. auto. progress; smt.
+  byequiv=> //=; proc.
+  inline CPA(BR,A).ARO.init CPA(BR1,A).ARO.init
+         CPA(BR,A).SO.kg CPA(BR1,A).SO.kg
+         CPA(BR,A).SO.enc CPA(BR1,A).SO.enc.
+  seq  9  9: (   ={glob A, glob RO, Log.qs, pk, sk, b, m, pk1}
+              /\ r{1} = BR1.r{2}
+              /\ (forall x, x \in Log.qs{1} <=> mem (dom RO.m){1} x)).
+  + auto. call (:   ={Log.qs, RO.m}
+                 /\ (forall x, x \in Log.qs{1} <=> mem (dom RO.m){1} x)).
+    + proc; inline RO.o.
+      auto=> /> &2 log_is_dom y _; smt (@NewFMap).
+    by inline *; auto=> />; rewrite dom0=> _ _ x; rewrite in_fset0.
+  (* Until the adversary queries the ROM with r, knowing that
+     the two ROMs agree on all points except r is sufficient
+     to prove the equivalence of the adversary's views        *)
+  call (_: mem Log.qs BR1.r ,
+           eq_except RO.m{1} RO.m{2} (pred1 BR1.r{2})).
+    (* Adversary is lossless *)
+  + exact/a2_ll.
+    (* Oracles are equivalent up to the failure event *)
+  + proc. inline RO.o.
+    auto=> /> &1 &2 -> /= m1_eqe_m2 yL y_in_dptxt; split.
+    + move=> x_notin_m; split.
+      + by rewrite !getP_eq eq_except_set.
+      move: m1_eqe_m2 x_notin_m=> + + + r_neq_x.
+      by rewrite eq_exceptP pred1E !in_dom=> /(_ x{2} r_neq_x) ->.
+    move=> x_in_m; split.
+    + move: m1_eqe_m2 x_in_m=> + + + r_neq_x.
+      by rewrite eq_exceptP pred1E !in_dom=> /(_ x{2} r_neq_x) ->.
+    by move: m1_eqe_m2=> + _ r_neq_x- /eq_exceptP /(_ x{2}); rewrite pred1E=> /(_ r_neq_x) ->.
+    (* Left oracle is lossless *)
+    move=> &2 _; exact/ARO_o_ll.
+    (* Right oracle is lossless and preserves bad once set *)
+    move=> _ /=; proc; inline *.
+    (* We simplify the goal by splitting it into:
+         1) the oracle is lossless; and
+         2) `bad` (`BR1.r \in Log.qs`) is monotonic. *)
+    conseq (: true ==> true: =1%r) (: BR1.r \in Log.qs ==> BR1.r \in Log.qs)=> //=.
+    + by auto=> />.
+    by auto=> />; exact/dptxt_ll.
+  (* We return to the main game *)
+  inline RO.o. case: ((mem (dom RO.m) r){1}).
+  + conseq (: _ ==> ={b} /\ BR1.r{2} \in Log.qs{2})=> //=.
+    + by move=> /> &1 &2 _ _ rR _ _ _ _ _ h /h [] -> //.
+    by auto=> /> &2 <- ->.
+  rcondt{1} 3; 1:by auto.
+  auto=> /> &2 log_is_dom r_notin_m y _; rewrite !getP_eq oget_some /=.
+  split.
+  + by move=> _; rewrite eq_exceptP /pred1=> x; rewrite getP=> ->.
+  by move=> _ rR aL mL aR qsR mR h /h [] ->.
   qed.
 
   (** Step 2: replace h ^ m with h in challenge encryption **)
@@ -245,22 +266,18 @@ section.
     Pr[CPA(BR1,A).main() @ &m: res]
     = Pr[CPA(BR2,A).main() @ &m: res].
   proof.
-    byequiv=> //=.
-    proc.
-    call (_: ={RO.m}).
-      proc. inline *. auto.
-    inline CPA(BR1,A).SO.enc CPA(BR2,A).SO.enc.
-    wp. rnd (fun x => m{2} +^ x).
-    rnd.
-    wp. rnd.
-    call (_: ={RO.m}).
-      proc. inline *. auto.
-    inline *. auto.
-    progress.
-      algebra.
-      smt.
-      smt.
-      algebra.
+  byequiv=> //=; proc.
+  call (_: ={RO.m}).
+  + by sim.
+  inline CPA(BR1,A).SO.enc CPA(BR2,A).SO.enc.
+  wp; rnd (fun x => m{2} +^ x).
+  auto; call (_: ={RO.m}).
+  + by sim.
+  inline *; auto=> /> _ _ rR bL _ rL _; split=> [|_].
+  + by move=> hR _; ring.
+  split=> [|_].
+  + by move=> hR _; exact/dptxt_funi.
+  by move=> hL _; rewrite dptxt_fu /=; ring.
   qed.
 
   (* The probability of the failure event is the same in both games *)
@@ -268,25 +285,20 @@ section.
     Pr[CPA(BR1,A).main() @ &m: mem Log.qs BR1.r]
     = Pr[CPA(BR2,A).main() @ &m: mem Log.qs BR2.r].
   proof.
-    byequiv=> //=.
-    proc.
-    call (_:    ={Log.qs, RO.m}
-             /\ BR1.r{1} = BR2.r{2}).
-      proc. inline *. auto.
-    inline CPA(BR1,A).SO.enc CPA(BR2,A).SO.enc.
-    wp. rnd (fun x => m{2} +^ x).
-    rnd. simplify.
-    wp. rnd.
-    call (_: ={Log.qs, RO.m}).
-      proc. inline *. auto.
-    inline *. auto.
-    progress.
-      algebra.
-      smt.
-      smt.
-      algebra.
+  byequiv=> //=; proc.
+  call (_:    ={Log.qs, RO.m}
+           /\ BR1.r{1} = BR2.r{2}).
+  + by sim.
+  inline CPA(BR1,A).SO.enc CPA(BR2,A).SO.enc.
+  wp; rnd (fun x => m{2} +^ x).
+  auto; call (_: ={Log.qs, RO.m}).
+  + by sim.
+  inline *; auto=> /> _ _ rR bL _ rL _; split=> [|_].
+  + by move=> hR _; ring.
+  split=> [|_].
+  + by move=> hR _; exact/dptxt_funi.
+  by move=> hL _; rewrite dptxt_fu /=; ring.
   qed.
-
   (** Exercise: What single "equiv" lemma could be used to prove both
       BR1_BR2 and BR1_BR2_bad in one? Prove it and use it to prove
       BR1_BR2_bad and BR1_BR2. **)
@@ -295,32 +307,29 @@ section.
     * exactly 1/2 **)
   local lemma pr_BR2_res &m: Pr[CPA(BR2,A).main() @ &m: res] = 1%r / 2%r.
   proof.
-    byphoare=> //=.
-    proc.
-    inline CPA(BR2, A).SO.enc.
-    swap 6 4; swap 4 5.
-    wp.
-    rnd (pred1 b')=> //=.
-    inline *.
-    call (_: true).
-      exact a2_ll. (* adversary *)
-      exact ARO_o_ll. (* oracle *)
-    auto.
-    call (_: true).
-      exact a1_ll. (* adversary *)
-      exact ARO_o_ll.
-    auto=> //=.
-    smt.
+  byphoare=> //=; proc.
+  inline CPA(BR2, A).SO.enc.
+  swap 6 4; swap 4 5.
+  wp; rnd (pred1 b')=> //=.
+  inline *; call (_: true).
+  + exact a2_ll. (* adversary *)
+  + exact ARO_o_ll. (* oracle *)
+  auto; call (_: true).
+  + exact a1_ll. (* adversary *)
+  + exact ARO_o_ll. (* oracle *)
+  auto=> />; rewrite dkeys_ll drand_ll dptxt_ll /predT /=.
+  by move=> _ _ _ _ _ _ r; rewrite dbool1E pred1E.
   qed.
 
   local lemma pr_BR_BR2 &m:
     Pr[CPA(BR,A).main() @ &m: res] - 1%r/2%r
     <= Pr[CPA(BR2,A).main() @ &m: mem Log.qs BR2.r].
-  proof. smt. qed.
+  proof. smt(BR_BR1 BR1_BR2 BR1_BR2_bad pr_BR2_res). qed.
 
   (** Step 3: Finally, we can do the reduction and prove that whenever
       A queries the RO with the randomness used in the challenge
       encryption, BR_OW(A) inverts the OW challenge. **)
+  (* We need a version of the one-way game where the challenge is a global *)
   local module OWr (I : Inverter) = {
     var x : rand
 
@@ -334,39 +343,41 @@ section.
     }
   }.
 
-  local lemma globx &m:
-    Pr[OW(BR_OW(A)).main() @ &m: res]
-    = Pr[OWr(BR_OW(A)).main() @ &m: res].
+  (* We can easily prove that it is strictly equivalent to OW *)
+  local lemma OW_OWr &m (I <: Inverter {OWr}):
+    Pr[OW(I).main() @ &m: res]
+    = Pr[OWr(I).main() @ &m: res].
   proof. by byequiv=> //=; sim. qed.
 
   local lemma BR2_OW &m:
     Pr[CPA(BR2,A).main() @ &m: mem Log.qs BR2.r]
     <= Pr[OW(BR_OW(A)).main() @ &m: res].
   proof.
-    rewrite (globx &m).
-    byequiv => //=.
-    proc; inline *; wp.
-    (* simplify postcondition to no longer have find *)
-    conseq [-frame]
-      (_ : _ ==>
-           support dkeys (pk0{2}, sk{2}) /\
-           BR2.r{1} = OWr.x{2} /\ Log.qs{1} = Log.qs{2} /\
-           y{2} = f pk0{2} BR2.r{1}).
-      progress; pose P := fun p => f _ p = _.
-      have h := nth_find witness P Log.qs{2} _.
-        by rewrite hasP; exists OWr.x{2}.
-      by rewrite (f_pk_inj _ _ _ _ H _ _ h) //; move=> _; rewrite Randomness.DWord.dunifin_fu.
-    (* rest of proof *)
-    swap {1} 3 - 2; swap {1} 9 -7; swap {1} 9 3; swap {1} 7 4.
-    wp. rnd{1}.
-    call (_: ={RO.m, Log.qs}); first by sim.
-    auto.
-    call (_: ={RO.m, Log.qs}); first by sim.
-    auto; smt.
+  rewrite (OW_OWr &m (BR_OW(A))).
+  byequiv => //=; proc; inline *; wp.
+  (* simplify postcondition to no longer have find *)
+  conseq
+    (_ : _ ==>
+         support dkeys (pk0{2}, sk{2}) /\
+         BR2.r{1} = OWr.x{2} /\ Log.qs{1} = Log.qs{2} /\
+         y{2} = f pk0{2} BR2.r{1}).
+  + move=> /> x qs pk sk vk x_in_qs; pose P := fun p => f _ p = _.
+    have h := nth_find witness P qs _.
+    + by rewrite hasP; exists x.
+    by rewrite (f_pk_inj _ _ _ _ vk _ _ h) // /f_dom drand_fu.
+  (* rest of proof *)
+  swap {1} 3 - 2; swap {1} 9 -7; swap {1} 9 3; swap {1} 7 4.
+  wp; rnd{1}.
+  call (_: ={RO.m, Log.qs}); first by sim.
+  auto.
+  call (_: ={RO.m, Log.qs}); first by sim.
+  by auto=> /> [pk sk] /= ->; rewrite dbool_ll.
   qed.
 
   lemma Reduction &m:
     Pr[CPA(BR,A).main() @ &m : res] - 1%r/2%r
     <= Pr[OW(BR_OW(A)).main() @ &m: res].
-  proof. smt. qed.
+  proof. smt(pr_BR_BR2 BR2_OW). qed.
 end section.
+
+print Reduction.
